attempt at unifying iEff_bottom with bottom effect signature

theories/logic/sem_types.v
@@ -121,40 +121,42 @@ Definition select_m (m : mode) (v : val) :=
   end.
 
 (* Effect Signature *)
-Definition sem_sig_eff_rec_pre {Σ} m (A B : sem_ty Σ -d> sem_sig Σ -d> sem_ty Σ) (rec : sem_sig Σ) : sem_sig Σ :=
-  (>> (α : sem_ty Σ) (a : val) >> ! (select_m m a) {{ ▷ (∃ rec', rec ≡ rec' ∧ A α rec' a) }}; 
+Definition sem_sig_eff_rec_pre `{!irisGS eff_lang Σ} m (A B : sem_ty Σ -d> sem_sig Σ -d> sem_ty Σ) (rec : sem_sig Σ) : sem_sig Σ :=
+  (>> (α : sem_ty Σ) (a : val) >> ! (select_m m a) {{ |={⊤}=> ▷ (∃ rec', rec ≡ rec' ∧ A α rec' a) }}; 
    << (b : val)                << ? b {{ ▷ (∃ rec', rec ≡ rec' ∧ B α rec' b) }} @m).
 
-Global Instance sem_sig_eff_rec_pre_contractive {Σ} m (A B : sem_ty Σ -d> sem_sig Σ -d> sem_ty Σ) :
+Global Instance sem_sig_eff_rec_pre_contractive `{irisGS eff_lang Σ} m (A B : sem_ty Σ -d> sem_sig Σ -d> sem_ty Σ) :
   Contractive (sem_sig_eff_rec_pre m A B).
 Proof.
   intros ?????. 
   rewrite /sem_sig_eff_rec_pre iEffPre_exist_eq iEffPost_exist_eq /=.
   intros ?. simpl. do 3 f_equiv. rewrite iEffPre_base_eq /=.
   intros ?. simpl. do 2 f_equiv.
-  { f_contractive. simpl in H. by do 4 f_equiv. }
+  { f_equiv. f_contractive. simpl in H. by do 4 f_equiv. }
   do 2 f_equiv. intros ?. rewrite /iEffPost_exist_def. do 3 f_equiv.
   rewrite iEffPost_base_eq /iEffPost_base_def. f_equiv. f_contractive.
   simpl in H. by do 4 f_equiv.
 Qed.
 
-Definition sem_sig_eff_rec {Σ} m (A B : sem_ty Σ → sem_sig Σ → sem_ty Σ) : sem_sig Σ :=
+Definition sem_sig_eff_rec `{irisGS eff_lang Σ} m (A B : sem_ty Σ → sem_sig Σ → sem_ty Σ) : sem_sig Σ :=
   fixpoint (sem_sig_eff_rec_pre m A B).
 
-Lemma sem_sig_eff_rec_unfold {Σ} m (A B : sem_ty Σ → sem_sig Σ → sem_ty Σ) `{NonExpansive2 A, NonExpansive2 B} :
+Lemma sem_sig_eff_rec_unfold `{irisGS eff_lang Σ} m (A B : sem_ty Σ → sem_sig Σ → sem_ty Σ) `{NonExpansive2 A, NonExpansive2 B} :
   (sem_sig_eff_rec m A B) ≡ 
-    (>> (α : sem_ty Σ) (a : val) >> ! (select_m m a) {{ ▷ (A α (sem_sig_eff_rec m A B) a) }}; 
+    (>> (α : sem_ty Σ) (a : val) >> ! (select_m m a) {{ |={⊤}=> ▷ (A α (sem_sig_eff_rec m A B) a) }}; 
      << (b : val)                << ? b {{ ▷ (B α (sem_sig_eff_rec m A B) b) }} @m)%ieff.
 Proof.
   rewrite {1} /sem_sig_eff_rec fixpoint_unfold {1} /sem_sig_eff_rec_pre.
   do 5 f_equiv. 
   - iSplit. 
-    + iIntros "[% [#Hfix HA]] !>". 
+    + iIntros "H". iMod "H". iIntros "!> !>". 
+      iDestruct "H" as "[% [#Hfix HA]]". 
       rewrite /sem_sig_eff_rec.
       iAssert (A a rec' ≡ A a (fixpoint (sem_sig_eff_rec_pre m A B)))%I as "#H".
       { by iRewrite "Hfix". }
       rewrite discrete_fun_equivI. by iRewrite - ("H" $! a0).
     + iIntros "HA //=". iExists (sem_sig_eff_rec m A B).
+      iMod "HA". iIntros "!> !>". 
       by iFrame. 
   - intros ?. rewrite iEffPost_base_eq /iEffPost_base_def.
     apply non_dep_fun_equiv. do 2 f_equiv. intros ?. do 2 f_equiv. iSplit.
@@ -167,22 +169,22 @@ Proof.
       by iFrame. 
 Qed.
 
-Lemma sem_sig_eff_rec_unfold' {Σ} m (A B : sem_ty Σ -d> sem_sig Σ -d> sem_ty Σ) `{ NonExpansive2 A, NonExpansive2 B } v Φ:
+Lemma sem_sig_eff_rec_unfold' `{irisGS eff_lang Σ} m (A B : sem_ty Σ -d> sem_sig Σ -d> sem_ty Σ) `{ NonExpansive2 A, NonExpansive2 B } v Φ:
   iEff_car (sem_sig_eff_rec m A B) v Φ ⊣⊢
-    iEff_car (>> (α : sem_ty Σ) (a : val) >> ! (select_m m a) {{ ▷ (A α (sem_sig_eff_rec m A B) a) }}; 
+    iEff_car (>> (α : sem_ty Σ) (a : val) >> ! (select_m m a) {{ |={⊤}=> ▷ (A α (sem_sig_eff_rec m A B) a) }}; 
               << (b : val)                << ? b {{ ▷ (B α (sem_sig_eff_rec m A B) b) }} @m)%ieff v Φ.
 Proof.
   assert (Hequiv :
   iEff_car (sem_sig_eff_rec m A B) v Φ ⊣⊢
-    iEff_car (>> (α : sem_ty Σ) (a : val) >> ! (select_m m a) {{ ▷ (A α (sem_sig_eff_rec m A B) a) }}; 
+    iEff_car (>> (α : sem_ty Σ) (a : val) >> ! (select_m m a) {{ |={⊤}=> ▷ (A α (sem_sig_eff_rec m A B) a) }}; 
               << (b : val)                << ? b {{ ▷ (B α (sem_sig_eff_rec m A B) b) }} @m)%ieff v Φ).
   { f_equiv. apply non_dep_fun_equiv. by apply sem_sig_eff_rec_unfold. }
   by rewrite Hequiv.
 Qed.
 
-Lemma sem_sig_eff_rec_eq {Σ} m A B v Φ `{ NonExpansive2 A, NonExpansive2 B }:
+Lemma sem_sig_eff_rec_eq `{irisGS eff_lang Σ} m A B v Φ `{ NonExpansive2 A, NonExpansive2 B }:
   iEff_car (sem_sig_eff_rec (Σ:=Σ) m A B) v Φ ⊣⊢
-    (∃ α a, ⌜ (select_m m a) = v ⌝ ∗ (▷ A α (sem_sig_eff_rec m A B) a) ∗ 
+    (∃ α a, ⌜ (select_m m a) = v ⌝ ∗ (|={⊤}=> ▷ A α (sem_sig_eff_rec m A B) a) ∗ 
                         □? m (∀ b, (▷ B α (sem_sig_eff_rec m A B) b) -∗ Φ b))%I.
 Proof. 
   etrans; [by apply sem_sig_eff_rec_unfold'|]. 
@@ -190,8 +192,8 @@ Proof.
 Qed.
 
 (* The sem_sig_eff_rec protocol is monotonic. *)
-Global Instance sem_sig_eff_rec_mono_prot {Σ} A B `{ NonExpansive2 A, NonExpansive2 B }:
-  MonoProt (@sem_sig_eff_rec Σ OS A B).
+Global Instance sem_sig_eff_rec_mono_prot `{irisGS eff_lang Σ} A B `{ NonExpansive2 A, NonExpansive2 B }:
+  MonoProt (@sem_sig_eff_rec Σ _ OS A B).
 Proof.
   constructor. iIntros (???) "HΦ'".
   rewrite !sem_sig_eff_rec_eq /=.
@@ -201,8 +203,8 @@ Proof.
 Qed.
 
 (* The sem_sig_eff_rec protocol is persistently monotonic. *)
-Global Instance sem_sig_eff_rec_pers_mono_prot {Σ} A B `{ NonExpansive2 A, NonExpansive2 B }:
-  PersMonoProt (@sem_sig_eff_rec Σ MS A B).
+Global Instance sem_sig_eff_rec_pers_mono_prot `{irisGS eff_lang Σ} A B `{ NonExpansive2 A, NonExpansive2 B }:
+  PersMonoProt (@sem_sig_eff_rec Σ _ MS A B).
 Proof.
   constructor. iIntros (???) "#HΦ'".
   rewrite !sem_sig_eff_rec_eq. simpl.
@@ -211,9 +213,9 @@ Proof.
   iIntros "!# %b Hκ". iApply "HΦ'". by iApply "HκΦ".
 Qed.
 
-Lemma upcl_sem_sig_rec_eff {Σ} m A B v Φ `{ NonExpansive2 A, NonExpansive2 B}:
+Lemma upcl_sem_sig_rec_eff `{irisGS eff_lang Σ} m A B v Φ `{ NonExpansive2 A, NonExpansive2 B}:
   iEff_car (upcl m (sem_sig_eff_rec (Σ:=Σ) m A B)) v Φ ⊣⊢
-    (∃ α a, ⌜ select_m m a = v ⌝ ∗ (▷ A α (sem_sig_eff_rec m A B) a) ∗ 
+    (∃ α a, ⌜ select_m m a = v ⌝ ∗ (|={⊤}=> ▷ A α (sem_sig_eff_rec m A B) a) ∗ 
                         □? m (∀ b, (▷ B α (sem_sig_eff_rec m A B) b) -∗ Φ b))%I.
 Proof.
   assert (Hequiv:
